\section{Proof of Lemma~\ref{lem:simple-reduction}}
\label{sec:proof-simple}

\SimpleReduction*


%old statement to go from local to global, no longer useful 
% \begin{lemma}
% 	\label{lem:local-to-global}
% 	If two protocols $\prot_1, \prot_2$ are such that for all local run $u_1$ of $\prot_1$, there is a local run $u_2$ of $\prot_2$ with the same initial values as $u_1$ and such that $\Input{u_1} = \Input{u_2}$ and $\Output{u_1} = \Output{u_2}$, then for all "boss specification" $bw \in \messages^*$, if $\prot_1$ has a run satisfying $\spec$ then so does $\prot_2$.
% \end{lemma}

% \cortoin{Only useful for the local equality test elimination}
% \ifproofs
% \begin{proof}
% 	We infer this statement from the "tree unfoldings".
	
% 	Suppose $\prot_1$ satisfies a specification $\spec$, then by Lemma~\ref{lem:run-to-tree} there exists a "tree unfolding" $\tree_1$ labelled by local runs of $\prot_1$ satisfying $\spec$. 
	
% 	Let $\node$ be a node of $\tree_1$ labelled by a "local run" $u_1$ of $\prot_1$, a value $v$ and a "specification" $\spec$.  
	
% 	There exists a "local run" $u_2$ of $\prot_2$ with the same initial values, "input" and "output" as $u_1$. In particular they have the same $v$-input and $v$-output.
	
% 	We define $\tree_2$ as the tree obtained by replacing in the label of each node the local run of $\prot_1$ by a local run of $\prot_2$ with the same initial values, "input" and "output". The rest of the labels stays the same.
	
% 	Conditions \ref{unfoldingC1}, \ref{unfoldingC2} and \ref{unfoldingC3} are still satisfied on every node as they only talk about the initial values, "input" and "output" of each local run label, and the value and specification labels. None of those things have changed.
% 	Furthermore as the specification label of the root is the same for $\tree_1$ and $\tree_2$, $\tree_2$ satisfies $\spec$.
	
% 	By Lemma~\ref{lem:tree-to-run}, as $\spec$ is a "boss specification", there exists a "run" of $\prot_2$ satisfying $\spec$.
% \end{proof}
% \fi

\begin{proof}
	We construct $\prot'$ as follows: It has one more register than $\prot$, but stores in its state the current state of $\prot$ and a mapping $map : \nset{1}{r} \to \nset{1}{r+1}$ from registers of $\prot$ to its own registers.
	
	Intuitively, it is going to use its registers to store the different values that are in the registers of $\prot$ and the mapping to keep track of which registers contain which values.
	When a value is received it guesses whether it is one of the existing values or a fresh one, and updates the registers and the mapping accordingly.
	The extra register of $\prot'$ is not necessary but simplifies the proof.
	For simplicity, we allow our system to have internal transitions with no effect (such transitions could be encoded using broadcasts with a dummy message type). 
	
	
	Let $\prot = (Q, \messages, \transitions', q_0, \regnum)$. 
	We define $\prot' := (Q', \messages, \transitions', q_0', \regnum +1)$ as follows. The set of states is $Q' := Q \times (\nset{1}{r} \to \nset{1}{r+1})$, its initial state is $q_0' := (q_0, \idmap)$ where $\idmap(i) = i$ for all $i \in \nset{1}{r}$. 
	
	The set of transitions $\transitions'$ is defined as follows.
	For all $q,q' \in Q$ and $\map, \map' \in \nset{1}{r} \to \nset{1}{r+1}$, we have $((q, \map), \op, (q', \map')) \in \transitions'$ in the following cases:
	
	\begin{itemize}
		\item $\op = \br{m}{j}$, 
		$\map = \map'$ and $(q, \br{m}{i}, q') \in \transitions$ for some $i$ such that $\map(i) = j$.
		
		\item $\op=\rec{m}{j}{\enregact}$, $\map^{-1}(j) =\emptyset$ and there is a transition $(q, \rec{m}{i_0}{\enregact}, q')$ in $\prot$ such that for all $i \in \nset{1}{r}$, if $i \ne i_0$ then $\map'(i) = \map(i)$ and $\map'(i_0) = j$.
		
		\item $\op = \rec{m}{j}{\eqtestact}$ and either
		\begin{itemize}
			\item there is a transition $(q, \rec{m}{i}, q') \in \transitions$ such that $\map(i)=j$ and $\map'=\map$.
			
			\item there is a transition $(q, \rec{m}{i_0}{\enregact}, q') \in \transitions$ such that $\map'(i_0)=j$ and $\map'(i) = \map(i)$ for every $i \neq i_0$.
		\end{itemize} 
		
		\item $\op = \rec{m}{j}{\diseqtestact}$ and there is a transition $(q, \rec{m}{i}{\diseqtestact}, q') \in \transitions$ such that $\map(i)=j$
		
		\item $\op=\loc{j_1}{j_2}{\diseqtestact}$ and there is a transition $(q, \loc{i_1}{i_2}{\diseqtestact}, q')$ such that $\map(i_1)=j_1$ and $\map(i_2) = j_2$.
	\end{itemize}
	
	
	We define the relation $\xrightarrow{\varepsilon}$ as $(q, map) \xrightarrow{\varepsilon} (q', map')$ if and only if $map=map'$ and there is a transition $q \xrightarrow{\loc{i_1}{i_2}{\eqtestact}} q'$ in $\prot$ such that $map(i_1)=j_1$ and $map(i_2) = j_2$.
	Let $\xrightarrow{\varepsilon}^*$ be its transitive closure.
	
	For all transitions $(q,map) \xrightarrow{\op} (q', map')$ we add transitions $(q,map) \xrightarrow{\op} (q'', map'')$ for all $q'', map''$ such that $(q', map') \xrightarrow{\varepsilon}^* (q'', map'')$, to obtain $\prot'$.
	
	We prove by induction on $\size{u}$ that for all "local run" $u$ of $\prot$ there exists a "local run" $u'$ of $\prot'$ with the same "trace" and such that if the last configuration of $u$ is $(q,\nu)$ and the last configuration of $u'$ is $((q',map), \nu')$ then $(q', map') \xrightarrow{\varepsilon}^* (q, map')$, for all $i$, $\nu(i) = \nu'(map(i))$ and for all $i_1, i_2$, if $\nu(i_1)=\nu_{i_2}$ then $map(i_1) = map(i_2)$.  
	
	If $\size{u} = 0$, let $(q_0, \nu_0)$ be its initial configuration, then we simply set $u'$ as an empty "local run" with the initial configuration $((q_0, id), \nu'_0)$ where $\nu'_0(i) = \nu_0(i)$ for all $i \in \nset{1}{r}$ and $\nu_0(r+1)$ is a fresh value.
	
	If $\size{u}>0$, let $\Tilde{u}$ be $u$ without its last step. Let $(q, \nu)$ be the last "local configuration" of $u$, $(\Tilde{q}, \Tilde{\nu})$ the one of $\Tilde{u}$.
	
	By induction hypothesis there exists $\Tilde{u}'$ a local run of $\prot'$ with the same "trace" to a "local configuration" $((\Tilde{q}', \Tilde{map}'), \Tilde{\nu}')$ such that $(\Tilde{q}', \Tilde{map}') \xrightarrow{\varepsilon}^* (\Tilde{q}, \Tilde{map}')$ and for all $i \in \nset{1}{r}$, $\Tilde{\nu}'(\Tilde{map}'(i)) = \Tilde{\nu}(i)$.
	
	\begin{itemize}
		\item 
		If the last step of $u$ is $(\Tilde{q}, \Tilde{\nu}) \xrightarrow{\br{m}{i}} (q, \nu)$ then $\Tilde{\nu} = \nu$, and there is a transition $(\Tilde{q}, \Tilde{map}') \xrightarrow{\br{m}{j}} (q, \Tilde{map}')$ with $j=\Tilde{map}'(i)$.
		
		We add a step $((\Tilde{q}', \Tilde{map}'), \Tilde{\nu}') \xrightarrow{\br{m}{j}} ((q', map'), \nu')$ at the end of $\Tilde{u}'$ to obtain $u'$, where $q' = q$, $map' = \Tilde{map}'$ and $\nu' = \Tilde{\nu}'$. 
		This step can be taken as $(\Tilde{q}', \Tilde{map}') \xrightarrow{\varepsilon}^* (\Tilde{q}, \Tilde{map}')$ and $(\Tilde{q}, \Tilde{map}') \xrightarrow{\br{m}{j}} (q, \Tilde{map}')$.   
		
		The resulting $u'$ satisfies the conditions as $(q', map') = (q, map')$, $\Tilde{map'} = map'$, the final configurations of $u$ and $u'$ are the same as the ones of $\Tilde{u}$ and $\Tilde{u}'$, and $\trace{u'} = \trace{\Tilde{u}'} (m,\Tilde{\nu}'(\Tilde{map}'(i)),out) = \trace{\Tilde{u}} (m,\Tilde{\nu}(i),out) = \trace{u}$.
		
		\item 
		If the last step of $u$ is an "external message" $(\Tilde{q}, \Tilde{\nu}) \extbr{m, v} (q, \nu)$ then let $j\in \nset{1}{r+1}$ be such that $\Tilde{map}'^{-1}(j) = \emptyset$ (such a $j$ exists as $\size{map(\nset{1}{r})} = r < r+1$). There is a transition $\Tilde{q} \xrightarrow{\rec{m}{i_0}{\alpha}} q$ in $\prot$ such that $\nu(i)=\Tilde{\nu}(i)$ for all $i\neq i_0$ and we are in one of the following cases:
		
		\begin{itemize}
			\item $\alpha=\enregact$, $\nu(i_0) = v$ and there exists $i_1 \neq i_0$ such that $\nu(i_1) = v$. Let $j_1=\Tilde{map}'(i_1)$
			There is a transition $(\Tilde{q}, \Tilde{map}') \xrightarrow{\rec{m}{j_1}{\eqtestact}} (q, map')$ in $\prot'$ with $map'(i) = \Tilde{map}'(i)$ for all $i\neq i_0$ and $map'(i_0) = j_1$.
			
			We add a step $((\Tilde{q}', \Tilde{map}'), \Tilde{\nu}') \extbr{m, v} ((q', map'), \nu')$ at the end of $\Tilde{u}'$ to obtain $u'$, where $q' = q$ and $\nu' = \Tilde{\nu}'$.
			
			This step can be taken as $(\Tilde{q}', \Tilde{map}') \xrightarrow{\varepsilon}^* (\Tilde{q}, \Tilde{map}')$ and $(\Tilde{q}', \Tilde{map}') \xrightarrow{\rec{m}{j_1}{\eqtestact}} (q', map')$. 
			
			We have $(q', map') = (q, map')$, $\nu'(map'(i_0)) = v = \nu(i_0)$ and $\nu'(map'(i)) = \Tilde{\nu}'(map'(i)) = \Tilde{\nu}(i) = \nu(i)$, and $\trace{u'} = \trace{\Tilde{u}'} (m,v,in) = \trace{\Tilde{u}} (m,v,in) = \trace{u}$.
			Furthermore for all $i', i'' \in \nset{1}{r}\setminus\set{i_0}$, if $\nu(i') = \nu(i'')$ then $map'(i') = \Tilde{map}'(i') = \Tilde{map}'(i'') = map'(i'')$, and for all $i' \in \nset{1}{r}$, if $\nu(i')=\nu(i_0)$ then $\nu(i')=\nu(i_1)$ and thus $map'(i') = map'(i_1) = map'(i_0)$.
			Thus the resulting $u'$ satisfies the conditions
			
			\item $\alpha=\enregact$, $\nu(i_0) = v$ and for all $i_1 \neq i_0$, $\nu(i_1) \neq v$. 
			There is a transition $(\Tilde{q}, \Tilde{map}') \xrightarrow{\rec{m}{j}{\enregact}} (q, map')$ in $\prot'$ with $map'(i) = \Tilde{map}'(i)$ for all $i\neq i_0$ and $map'(i_0) = j$.
			
			We add a step $((\Tilde{q}', \Tilde{map}'), \Tilde{\nu}') \extbr{m, v} ((q', map'), \nu')$ at the end of $\Tilde{u}'$ to obtain $u'$, where $q' = q$ and $\nu'(j') = \Tilde{\nu}'(j')$ for all $j' \neq j$ and $\nu'(j) = v$.
			
			This step can be taken as $(\Tilde{q}', \Tilde{map}') \xrightarrow{\varepsilon}^* (\Tilde{q}, \Tilde{map}')$ and $(\Tilde{q}', \Tilde{map}') \xrightarrow{\rec{m}{j}{\enregact}} (q', map')$. 
			
			The resulting $u'$ satisfies the conditions as $(q', map') = (q, map')$, we have $\nu'(map'(i_0)) = v = \nu(i_0)$ and $\nu'(map'(i)) = \Tilde{\nu}'(map'(i)) = \Tilde{\nu}(i) = \nu(i)$, and $\trace{u'} = \trace{\Tilde{u}'} (m,v,in) = \trace{\Tilde{u}} (m,v,in) = \trace{u}$.
			
			\item $\alpha = \eqtestact$, $\nu(i_0) = \Tilde{\nu}(i_0) = v$. Then there is a transition $(\Tilde{q}, \Tilde{map}') \xrightarrow{\rec{m}{j}{\eqtestact}} (q, map')$ in $\prot'$ with $map' = \Tilde{map}'$ and $j = \Tilde{map}'(i_0)$.
			
			We add a step $((\Tilde{q}', \Tilde{map}'), \Tilde{\nu}') \extbr{m, v} ((q', map'), \nu')$ at the end of $\Tilde{u}'$ to obtain $u'$, where $q' = q$ and $\nu' = \Tilde{\nu}'$.
			
			This step can be taken as $\Tilde{\nu}'(\Tilde{map}'(i)) = \Tilde{\nu}(i) = v$ and $(\Tilde{q}', \Tilde{map}') \xrightarrow{\varepsilon}^* (\Tilde{q}, \Tilde{map}')$ and $(\Tilde{q}', \Tilde{map}') \xrightarrow{\rec{m}{j}{\eqtestact}} (q', map')$.
			
			The resulting $u'$ satisfies the conditions as $(q', map') = (q, map')$, the final configurations of $u$ and $u'$ are the same as the ones of $\Tilde{u}$ and $\Tilde{u}'$, and $\trace{u'} = \trace{\Tilde{u}'} (m,v,in) = \trace{\Tilde{u}} (m,v,in) = \trace{u}$.
			
			\item $\alpha = \diseqtestact$ and $\nu(i_0) = \Tilde{\nu}(i_0) \neq v$. Then there is a transition $(\Tilde{q}, \Tilde{map}') \xrightarrow{\rec{m}{j}{\diseqtestact}} (q, map')$ in $\prot'$ with $map' = \Tilde{map}'$ and $j = \Tilde{map}'(i_0)$.
			
			We add a step $((\Tilde{q}', \Tilde{map}'), \Tilde{\nu}') \extbr{m, v} ((q', map'), \nu')$ at the end of $\Tilde{u}'$ to obtain $u'$, where $q' = q$ and $\nu' = \Tilde{\nu}'$.
			
			This step can be taken as $\Tilde{\nu}'(\Tilde{map}'(i)) = \Tilde{\nu}(i) \neq v$ and $(\Tilde{q}', \Tilde{map}') \xrightarrow{\varepsilon}^* (\Tilde{q}, \Tilde{map}')$ and $(\Tilde{q}', \Tilde{map}') \xrightarrow{\rec{m}{j}{\diseqtestact}} (q', map')$.
			
			The resulting $u'$ satisfies the conditions as $(q', map') = (q, map')$, the final configurations of $u$ and $u'$ are the same as the ones of $\Tilde{u}$ and $\Tilde{u}'$, and $\trace{u'} = \trace{\Tilde{u}'} (m,v,in) = \trace{\Tilde{u}} (m,v,in) = \trace{u}$.
			
			\item $\alpha = \dummyact$ and $\nu(i_0) = \Tilde{\nu}(i_0)$. Then there is a transition $(\Tilde{q}, \Tilde{map}') \xrightarrow{\rec{m}{j}{\enregact}} (q, map')$ in $\prot'$ with $map' = \Tilde{map}'$.
			
			We add a step $((\Tilde{q}', \Tilde{map}'), \Tilde{\nu}') \extbr{m, v} ((q', map'), \nu')$ at the end of $\Tilde{u}'$ to obtain $u'$, where $q' = q$ and $\nu' = \Tilde{\nu}'$.
			
			This step can be taken as $(\Tilde{q}', \Tilde{map}') \xrightarrow{\varepsilon}^* (\Tilde{q}, \Tilde{map}')$ and $(\Tilde{q}', \Tilde{map}') \xrightarrow{\rec{m}{j}{\enregact}} (q', map')$.
			
			The resulting $u'$ satisfies the conditions as $(q', map') = (q, map')$, the final configurations of $u$ and $u'$ are the same as the ones of $\Tilde{u}$ and $\Tilde{u}'$, and $\trace{u'} = \trace{\Tilde{u}'} (m,v,in) = \trace{\Tilde{u}} (m,v,in) = \trace{u}$. 
		\end{itemize}
		
		\item 
		If the last step of $u$ is $(\Tilde{q}, \Tilde{\nu}) \xrightarrow{\loc{i_1}{i_2}{\eqtestact}} (q, \nu)$ then $\Tilde{\nu} = \nu$, and $(\Tilde{q}, \Tilde{map}') \xrightarrow{\varepsilon} (q, \Tilde{map}')$.
		
		We set $u' = \Tilde{u}'$. The last configuration of $u'$ is $((\Tilde{q}', \Tilde{map}'), \Tilde{\nu}')$. It satisfies the conditions as $(\Tilde{q}', \Tilde{map}') \xrightarrow{\varepsilon}^* (\Tilde{q}, \Tilde{map}') \xrightarrow{\varepsilon} (q, \Tilde{map}')$ and the final configurations of $u$ and $u'$ are the same as the ones of $\Tilde{u}$ and $\Tilde{u}'$.
		
		\item 
		If the last step of $u$ is $(\Tilde{q}, \Tilde{\nu}) \xrightarrow{\loc{i_1}{i_2}{\diseqtestact}} (q, \nu)$ then $\Tilde{\nu} = \nu$, and there is a transition $(\Tilde{q}, \Tilde{map}') \xrightarrow{\loc{j_1}{j_2}{\diseqtestact}} (q, \Tilde{map}')$ with $j_1=\Tilde{map}'(i_1)$ and $j_2=\Tilde{map}'(i_2)$.
		
		We add a step $((\Tilde{q}', \Tilde{map}'), \Tilde{\nu}') \xrightarrow{\loc{j_1}{j_2}{\diseqtestact}} ((q', map'), \nu')$ at the end of $\Tilde{u}'$ to obtain $u'$, where $q' = q$, $map' = \Tilde{map}'$ and $\nu' = \Tilde{\nu}'$. 
		This step can be taken as $\Tilde{\nu}'(j_1) = \Tilde{\nu}(i_1) \neq \Tilde{\nu}(i_2) = \Tilde{\nu}'(j_2)$ and $(\Tilde{q}', \Tilde{map}') \xrightarrow{\varepsilon}^* (\Tilde{q}, \Tilde{map}')$ and $(\Tilde{q}, \Tilde{map}') \xrightarrow{\loc{j_1}{j_2}{\diseqtestact}} (q, \Tilde{map}')$.   
		
		The resulting $u'$ satisfies the conditions as $(q', map') = (q, map')$ and the "traces" and final configurations of $u$ and $u'$ are the same as the ones of $\Tilde{u}$ and $\Tilde{u}'$.
	\end{itemize}
	
	This concludes our first induction.
	
	We now prove by induction on $\size{u'}$ that for all "local run" $u'$ of $\prot'$ there exists a "local run" $u$ of $\prot$ with the same "trace" and such that if the last configuration of $u$ is $(q,\nu)$ and the last configuration of $u'$ is $((q',map), \nu')$ then $q=q'$ and for all $i$, $\nu(i) = \nu'(map(i))$.  
	
	If $\size{u'} = 0$, let $(q_0, \nu'_0)$ be its initial configuration, then we  set $u$ as an empty "local run" with the initial configuration $((q_0, id), \nu_0)$ where $\nu_0(i) = \nu'_0(i)$ for all $i \in \nset{1}{r}$.
	
	If $\size{u}>0$, let $\Tilde{u}'$ be $u'$ without its last step. Let $((q', map'), \nu')$ be the last "local configuration" of $u'$, $((\Tilde{q}', \Tilde{map}'), \Tilde{\nu}')$ the one of $\Tilde{u}'$.
	
	By induction hypothesis there exists $\Tilde{u}$ a local run of $\prot$ with the same "trace" as $u'$ to a "local configuration" $(\Tilde{q}, \Tilde{\nu})$ such that $\Tilde{q}'=\Tilde{q}$ and for all $i \in \nset{1}{r}$, $\Tilde{\nu}'(\Tilde{map}'(i)) = \Tilde{\nu}(i)$.
	
	\begin{itemize}
		\item If the last step of $u'$ is $((\Tilde{q}', \Tilde{map}'), \Tilde{\nu}') \xrightarrow{\br{m}{j}} ((q', map'), \nu')$, then $\Tilde{map}' = map'$ and there exists $q \in Q$ and $i \in \nset{1}{r}$ such that $map'(i)=j$ and $(\Tilde{q}, map') \xrightarrow{\varepsilon}^* (q, map')$ and $q \xrightarrow{\br{m}{i}} q'$ is a transition of $\prot$.
		
		As $(\Tilde{q}, map') \xrightarrow{\varepsilon}^* (q, map')$ and $map'=\Tilde{map}'$, there is a path in $\prot$ from $\Tilde{q}$ to $q$ consisting only of transitions labelled by operations of the form $\loc{i_1}{i_2}{\eqtestact}$ with $\Tilde{map}'(i_1) = \Tilde{map}'(i_2)$ and thus $\Tilde{\nu}(i_1) = \Tilde{\nu}(i_2)$.
		As a result, we can extend $\Tilde{u}$ into a "local run" to $(q, \Tilde{\nu})$ with the same  "trace" as $\Tilde{u}$.
		
		We then append a step $(q, \Tilde{\nu}) \xrightarrow{\br{m}{i}} (q', \nu)$ at the end of that local run to obtain $u$. As $j = map(i)$, we have $\Tilde{\nu}(i) = \Tilde{\nu}'(j)$ and thus $\trace{u} = \trace{\Tilde{u}}(m, \Tilde{\nu}(i), out) = \trace{\Tilde{u}'}(m, \Tilde{\nu}'(j), out) = \trace{u'}$.
		
		\item If the last step of $u'$ is $((\Tilde{q}', \Tilde{map}'), \Tilde{\nu}') \extbr{m, v} ((q', map'), \nu')$, then there exists a transition  $(\Tilde{q}', \Tilde{map}') \xrightarrow{\rec{m}{j_0}{\alpha}} (q', map')$ and $i_0 \in \nset{1}{r}$ such that $map'(i) = \Tilde{map}'(i)$ for all $i\neq i_0$ and we are in one of the following cases:
		
		\begin{itemize}
			\item $\alpha = \enregact$ and $\nu'(j_0)=v$. Then there exists $q \in Q$ and $i \in \nset{1}{r}$ such that $(\Tilde{q}, map') \xrightarrow{\varepsilon}^* (q, map')$ and $q \xrightarrow{\rec{m}{i_0}{\beta}} q'$ is a transition of $\prot$
			
			Like before, as $(\Tilde{q}, map') \xrightarrow{\varepsilon}^* (q, map')$ and $map'=\Tilde{map}'$, we can extend $\Tilde{u}$ into a "local run" to $(q, \Tilde{\nu})$ with the same  "trace" as $\Tilde{u}$.
			
			We have either
			\begin{itemize}
				\item $\beta=\enregact$ and $map'(i_0) = j_0$. Then we add a step $(q, \Tilde{\nu}) \extbr{m,v} (q', \nu)$ at the end of the constructed local run to obtain $u$, with $\nu(i_0)=v$ and $\nu(i) = \Tilde{\nu}(i)$ for all $i \neq i_0$.
				
				\item $\beta=\dummyact$ and $map' = \Tilde{map}'$. Then we add a step $(q, \Tilde{\nu}) \extbr{m,v} (q', \nu)$ at the end of the constructed local run to obtain $u$, with $\nu = \Tilde{\nu}$.
			\end{itemize}
			
			\item $\alpha = \eqtestact$ and $map'(i_0)=\Tilde{map}'(i_0)$ and $\nu'(j_0) = \Tilde{\nu}'(j_0) = v$. Then there exists $q \in Q$ such that $(\Tilde{q}, map') \xrightarrow{\varepsilon}^* (q, map')$ and $q \xrightarrow{\rec{m}{i_0}{\beta}} q'$ is a transition of $\prot$.
			
			Like before, as $(\Tilde{q}, map') \xrightarrow{\varepsilon}^* (q, map')$ and $map'=\Tilde{map}'$, we can extend $\Tilde{u}$ into a "local run" to $(q, \Tilde{\nu})$ with the same  "trace" as $\Tilde{u}$.
			
			We have either
			\begin{itemize}
				\item $\beta=\eqtestact$ and $map' = \Tilde{map}'$ and $\Tilde{\nu}(i_0) = v$. Then we add a step $(q, \Tilde{\nu}) \extbr{m,v} (q', \nu)$ at the end of the constructed local run to obtain $u$, with $\nu = \Tilde{\nu}$.
				
				\item $\beta=\enregact$. Then we add a step $(q, \Tilde{\nu}) \extbr{m,v} (q', \nu)$ at the end of the constructed local run to obtain $u$, with $\nu(i_0) = v$ and $\nu(i)=\Tilde{\nu}(i)$ for all $i \neq i_0$.
			\end{itemize}
			
			\item $\alpha = \diseqtestact$ and $map'(i_0)=\Tilde{map}'(i_0) \neq v$. Then there exists $q \in Q$ and $i_0 \in \nset{1}{r}$ such that $(\Tilde{q}, map') \xrightarrow{\varepsilon}^* (q, map')$ and $q \xrightarrow{\rec{m}{i_0}{\diseqtestact}} q'$ is a transition of $\prot$.
			
			Like before, as $(\Tilde{q}, map') \xrightarrow{\varepsilon}^* (q, map')$ and $map'=\Tilde{map}'$, we can extend $\Tilde{u}$ into a "local run" to $(q, \Tilde{\nu})$ with the same "trace" as $\Tilde{u}$.
			
			We add a step $(\Tilde{q}, \Tilde{\nu}) \extbr{m,v} (q, \nu)$ at the end to obtain $u$, with $\nu = \nu'$.
		\end{itemize}
		
		In all cases, the conditions are respected, as $\trace{u} = \trace{\Tilde{u}} (m,v, in) = \trace{\Tilde{u}'} (m,v, in) = \trace{u'}$.
		
		\item If the last step of $u'$ is $((\Tilde{q}', \Tilde{map}'), \Tilde{\nu}') \xrightarrow{\loc{j_1}{j_2}{\diseqtestact}} ((q', map'), \nu')$ then $map'=\Tilde{map}'$, $\nu' = \Tilde{\nu}'$, $\nu'(j_1) \neq \nu'(j_2)$ and there exists $q \in Q$ and $i_1, i_2 \in \nset{1}{r}$ such that $map'(i_1)=j_1$, $map'(i_2)=j_2$ and $(\Tilde{q}, map') \xrightarrow{\varepsilon}^* (q, map')$ and $q \xrightarrow{\loc{i_1}{i_2}{\diseqtestact}} q'$ is a transition of $\prot$.
		
		Like before, as $(\Tilde{q}, map') \xrightarrow{\varepsilon}^* (q, map')$ and $map'=\Tilde{map}'$, we can extend $\Tilde{u}$ into a "local run" to $(q, \Tilde{\nu})$ with the same "trace" as $\Tilde{u}$.
		
		
		We append a step $(q, \Tilde{\nu}) \xrightarrow{\loc{i_1}{i_2}{\diseqtestact}} (q', \nu)$ at the end of that local run to obtain $u$, with $\nu = \Tilde{\nu}$. We have $\Tilde{\nu}(i_1) = \Tilde{\nu}'(j_1) \neq \Tilde{\nu}'(j_2) = \Tilde{\nu}(i_2)$ and thus $\trace{u} = \trace{\Tilde{u}} = \trace{\Tilde{u}'} = \trace{u'}$.
	\end{itemize}
	
	We have shown that $\prot$ and $\prot'$ produce the same set of "traces" from their "local runs". As the "input" and "output" of a local run depend only on its "trace", we obtain the result by Lemma~\ref{lem:local-to-global}.
\end{proof}
